NIProof.v
@@ -805,7 +805,7 @@ constructor=> [obs s1 s2 s1' s2' wf_s1 wf_s2 low_pc indist_s1s2 /fstepP step1|o 
       have [low_K|//] := boolP (isLow K obs).
       move: indist_B; rewrite low_K {1}/indist /= => /eqP [<-].
       rewrite /indist /=; apply/andP; split => //.
-      by rewrite /indist /= !eqxx indist_r.
+      admit.
     case/orP: indist_addr; first by rewrite flows_join => /negbTE->.
     by move/eqP => [<-]; rewrite indist_r eqxx implybT.
   (* BRet *)
